Start steps-to relation

theory/Inet.v
@@ -10,7 +10,7 @@ Open Scope list_scope.
 (* Default notation for vectors overrides list notation. Redefine it *)
 Notation "'<<' '>>'" := (Vector.nil _) (at level 60, right associativity).
 Notation "h <::> t" := (Vector.cons _ h _ t) (at level 60, right associativity).
-Notation "< x >" := (x <::> <<>>).
+Notation "<< x >>" := (x <::> <<>>).
 Notation "<< x ; y ; .. ; z >>" := 
   (Vector.cons _ x _ (Vector.cons _ y _ .. (Vector.cons _ z _ 
   (Vector.nil _)) ..)).
@@ -36,19 +36,21 @@ Inductive term : Type :=
   | tree : forall arity : nat,
       agent arity -> VectorDef.t term arity -> term.
 
+Arguments tree {arity}.
+
 Check leaf "alpha".
-Check tree 2 "alpha" << leaf "beta"; leaf "gamma" >>.
-Fail Check tree 1 "alpha" << leaf "beta"; leaf "gamma" >>.
+Check tree "alpha" << leaf "beta"; leaf "gamma" >>.
+Fail Check @tree 3 "alpha" << leaf "beta"; leaf "gamma" >>.
 
 Fixpoint names_of_term (t : term) : list string :=
   match t with
   | leaf n => [n]
-  | tree _ _ terms => 
+  | tree  _ terms => 
       List.concat (Vector.to_list (Vector.map names_of_term terms))
   end.
 
 Compute names_of_term (leaf "alpha").
-Compute names_of_term (tree 2 "alpha" << leaf "beta"; leaf "gamma" >>).
+Compute names_of_term (tree "alpha" << leaf "beta"; leaf "gamma" >>).
 
 (* Renaming and Substitution *)
 Reserved Notation "'[[' x ':=' u ']]' t" (at level 20).
@@ -59,18 +61,18 @@ Fixpoint subst (t : term) (x : string) (u : term) : term :=
         u
       else
         t
-  | tree arity agent terms =>
-      tree arity agent (Vector.map (fun t =>
+  | tree agent terms =>
+      tree agent (Vector.map (fun t =>
         [[x := u]] t
       ) terms)
   end
 where "'[[' x ':=' u ']]' t" := (subst t x u).
 
 Compute [["x" := leaf "y"]] (leaf "x").
-Compute [["x" := tree 2 "x" << leaf "y"; leaf "z" >>]] (
-  tree 2 "alpha" <<
+Compute [["x" := tree "x" << leaf "y"; leaf "z" >>]] (
+  tree "alpha" <<
     leaf "x";
-    tree 3 "beta" <<
+    tree "beta" <<
       leaf "x";
       leaf "y";
       leaf "z"
@@ -78,39 +80,63 @@ Compute [["x" := tree 2 "x" << leaf "y"; leaf "z" >>]] (
   >>
 ).
 
-(* Rules *)
-Axiom rule : relation term.
-Definition interacts_with (t1 : term) (t2 : term) : Prop := rule t1 t1.
+Compute [["y" := leaf "v"]] ([["x" := leaf "u"]] (leaf "y")).
+Compute [["x" :=  [["y" := leaf "v"]] leaf "u"]] (leaf "y").
 
+(* Rules *)
+Inductive interacts_with : term -> term -> Prop :=
+  | rule : forall t1 t2, interacts_with t1 t2.
 Notation "t1 '⋈' t2" := (interacts_with t1 t2) (at level 60, right associativity).
 
 Check (leaf "alpha") ⋈ (leaf "beta").
-Check (tree 2 "alpha" << leaf "beta"; leaf "gamma" >>) ⋈ (leaf "beta").
-Check [ (leaf "alpha") ⋈ (leaf "beta");
-        (tree 2 "alpha" << leaf "beta"; leaf "gamma" >>) ⋈ (leaf "beta")
-      ].
+Check (tree "alpha" << leaf "beta"; leaf "gamma" >>) ⋈ (leaf "beta").
   
+(* Define some agents *)
+Definition x := leaf "x".
+Definition y := leaf "y".
+Definition t := leaf "t".
+Definition O := tree "O" (<<>>).
+Definition S (n : term) := tree "S" <<n>>.
+Definition add (x : term) (y : term) := tree "add" << x ; y >>.
 
-(* Equations *)
-Definition eqn (X : Type) : Type := X -> X -> Prop.
+Definition add_O := O ⋈ add y y.
+Definition add_S := S (add y t) ⋈ add y (S t).
 
-(* Configurations *)
-Record conf : Type := mkconf {
-  interface : list term;
-  equations: list (eqn term);
-}.
+Inductive unify : term -> term -> Prop :=
+  | goal : forall t1 t2, unify t1 t2.
+Notation "t1 ~= t2" := (unify t1 t2) (at level 60, right associativity).
 
-(* Interaction rules *)
-(* TODO *)
+Definition eqn : Type := term * term.
 
-(* Nets *)
-(* TODO *)
+Fixpoint combine_vecs_to_list {X : Type} {n : nat} (a : VectorDef.t X n)
+  (b : VectorDef.t X n) :=
+  let xs := Vector.to_list a in
+  let ys := Vector.to_list b in
+  List.combine xs ys.
 
-(* Steps-to relation on configurations *)
-(*
-Inductive steps_to : conf -> conf -> Prop :=
-  | interaction
-  | indirection
-  | collect
-  | multiset.
-*)
+Notation "xs <*> ys" := (combine_vecs_to_list xs ys) (at level 60, right associativity).
+
+Inductive steps_to : list eqn -> list eqn -> Prop :=
+  | interaction :
+      forall m n a b xs xs' ys ys' (Γ : list eqn),
+      @tree m a xs ⋈ @tree n b ys ->
+      @tree m a xs' ~= @tree n b ys' ->
+      steps_to ((@tree m a xs', @tree n b ys') :: Γ)
+      ((xs <*> xs') ++ (ys <*> ys') ++ Γ).
+
+Lemma steps_to_example : 
+  add_O ->
+  O ~= add (leaf "1") (leaf "1") ->
+  steps_to 
+    [(O, add (leaf "1") (leaf "1"))]
+    (
+      (<<>> <*> <<>>) ++
+      (<<leaf "y"; leaf "y">> <*> <<leaf "1"; leaf "1">>) ++
+      []
+    ).
+Proof.
+  intros.
+  apply interaction.
+  - unfold add_O in H. apply H.
+  - apply H0.
+Qed.
